expr_adversarial {t1 t2} (_:expr t1) : expr t2
Switch back to polymorphic adversaries.
We used to do this, but switched to fixed-type adversaries because
implementing adveraries required typecase, which was doable but painful.
Now it seems that needing to convert all adversary inputs and outputs to
the distinguished message type is even more painful.

src/Minimalistic.v
@@ -19,7 +19,7 @@ Section Language.
   Inductive expr : type -> Type :=
   | expr_const {t} (_:forall eta, interp_type t eta) : expr t
   | expr_random (idx:positive) : expr trand
-  | expr_adversarial (_:expr (tlist tmessage)) : expr tmessage
+  | expr_adversarial {t1 t2} (_:expr t1) : expr t2
   | expr_app {t1 t2} (_:(t1 -> t2)%etype) (_:expr t1) : expr t2
   | expr_pair {t1 t2} (_:expr t1) (_:expr t2) : expr (t1 * t2).
 
@@ -28,8 +28,9 @@ Section Language.
 
   Local Notation "'#' x" := (expr_const x) (right associativity, at level 9, format "# x") : expr_scope.
   Local Notation "'$' x" := (expr_random x%positive) (right associativity, at level 79, x at next level, format "$ x") : expr_scope. (* FIXME: we want level 9, but it conflicts with fcf *)
-  Local Notation "'!' '@' x" := (expr_adversarial x%expr) (left associativity, at level 11, format "! @ x").
   Local Notation "f @ x" := (expr_app f x) (left associativity, at level 11, format "f @ x").
+  Local Notation "'!' '@' x" := (expr_adversarial x%expr) (left associativity, at level 11, format "! @ x").
+  Local Notation "'!' t '@' x" := (@expr_adversarial _ t x%expr) (left associativity, at level 11, format "! t @ x", t at next level).
   Local Notation "( x , y , .. , z )" := (expr_pair .. (expr_pair x%expr y%expr) .. z%expr) : expr_scope.
 
   Fixpoint randomness_indices {t:type} (e:expr t) : PositiveSet.t :=
@@ -245,13 +246,13 @@ Section Language.
   Arguments interp_pair {_ _ _}.
 
   Fixpoint interp_fixed {t} (e:expr t) (eta : nat)
-           (adv: interp_type (tlist tmessage) eta -> interp_type tmessage eta)
+           (adv: forall t1 t2, interp_type t1 eta -> interp_type t2 eta)
            (rands: PositiveMap.t (interp_type trand eta))
     : interp_type t eta :=
     match e with
     | # c => c eta
     | $ i => match PositiveMap.find i rands with Some r => r | _ => cast_rand eta (Bvector_exists _) end
-    | !@inputs => adv (interp_fixed inputs eta adv rands)
+    | !@inputs => adv _ _ (interp_fixed inputs eta adv rands)
     | f@inputs => interp_func f (interp_fixed inputs eta adv rands)
     | (a, b) => interp_pair (interp_fixed a eta adv rands) (interp_fixed b eta adv rands)
     end%expr.
@@ -273,11 +274,11 @@ Section Language.
     (* the adversary is split into three parts for no particular reason. It first decides how much randomness it will need, then interacts with the protocol (repeated calls to [adversary] with all messages up to now as input), and then tries to claim victory ([distinguisher]). There is no explicit sharing of state between these procedures, but all of them get the same random inputs in the security game. The handling of state is a major difference between FCF [OracleComp] and this framework *)
     Definition universal_security_game {t}
                (evil_rand_indices: forall eta:nat, PositiveSet.t)
-               (adversary:forall (eta:nat) (rands: PositiveMap.t (interp_type trand eta)), interp_type (tlist tmessage) eta -> interp_type tmessage eta)
+               (adv:forall (eta:nat) (rands: PositiveMap.t (interp_type trand eta)) t1 t2, interp_type t1 eta -> interp_type t2 eta)
                (distinguisher: forall (eta:nat) (rands: PositiveMap.t (interp_type trand eta)), interp_type t eta -> Datatypes.bool)
                (eta:nat) (e:expr t) : Comp Datatypes.bool :=
       evil_rands <-$ generate_randomness eta (evil_rand_indices eta);
-        out <-$ interp e eta (adversary eta (evil_rands));
+        out <-$ interp e eta (adv eta (evil_rands));
         ret (distinguisher eta evil_rands out).
 
     Definition indist {t:type} (a b:expr t) : Prop :=  forall adl adv dst,
@@ -1471,7 +1472,7 @@ Section Language.
              end.
     Qed.
 
-    Global Instance Proper_eqwhp_adversarial : Proper (eqwhp ==> eqwhp) expr_adversarial.
+    Global Instance Proper_eqwhp_adversarial {t1 t2} : Proper (eqwhp ==> eqwhp) (@expr_adversarial t1 t2).
     Proof.
       intros ??.
       eapply whp_impl.
@@ -1505,7 +1506,7 @@ Section Language.
   Section LateInterp.
     Fixpoint interp_late
              {t} (e:expr t) (eta : nat)
-             (adv: interp_type (tlist tmessage) eta -> interp_type tmessage eta)
+             (adv: forall t1 t2, interp_type t1 eta -> interp_type t2 eta)
              (fixed_rand: PositiveMap.t (interp_type trand eta))
     : Comp (interp_type t eta) :=
       match e with
@@ -1516,7 +1517,7 @@ Section Language.
         | _ => r <-$ {0,1}^eta; ret (cast_rand eta r)
         end
       | !@ctx =>
-        ctx <-$ interp_late ctx eta adv fixed_rand; ret (adv ctx)
+        ctx <-$ interp_late ctx eta adv fixed_rand; ret (adv _ _ ctx)
       | f@x =>
         x <-$ interp_late x eta adv fixed_rand; ret (interp_func f x)
       | (a, b) =>
@@ -1641,7 +1642,7 @@ Section Language.
     destruct b; rewrite eqb_refl; reflexivity.
   Qed.
 
-  Context (vmessage_exists : forall eta, interp_type tmessage eta).
+  Context (inhabited : forall t eta, interp_type t eta).
 
   (* TODO: contribute to FCF *)
   Lemma not_negligible_const c (Hc: ~ c == 0) : ~ negligible (fun _ => c).
@@ -1666,7 +1667,7 @@ Section Language.
     cbv [indist universal_security_game interp].
     intro H.
     specialize (H (fun _ => PositiveSet.empty)
-                  (fun _ _ _ => (vmessage_exists _))
+                  (fun n _ _ t _ => inhabited t n)
                   (fun eta rands v => inspect_vbool v)).
     cbv [id] in *.
     setoid_rewrite Bind_unused in H.
@@ -1728,7 +1729,7 @@ Section Language.
     (* boring recursion: *)
     | ssconst t v : @signature_safe sk t #v nil
     | ssfunc {t1 t2} (f : func t1 t2) e S : signature_safe sk e S -> signature_safe sk (f@e) S
-    | ssadv                           e S : signature_safe sk e S -> signature_safe sk (!@e) S
+    | ssadv  {t1 t2} (e : expr t1) S : signature_safe sk e S -> signature_safe sk (!t2@e) S
     | sspair {t1 t2} (e1: expr t1) (e2: expr t2) S1 S2 :
         signature_safe sk e1 S1 ->
         signature_safe sk e2 S2 ->
@@ -1759,7 +1760,7 @@ Section Language.
     (* boring recursion: *)
     | msconst t v : @mac_safe sk t #v nil
     | msfunc {t1 t2} (f : func t1 t2) e S : mac_safe sk e S -> mac_safe sk (f@e) S
-    | msadv                           e S : mac_safe sk e S -> mac_safe sk (!@e) S
+    | msadv  {t1 t2} (e : expr t1) S : mac_safe sk e S -> mac_safe sk (!t2@e) S
     | mspair {t1 t2} (e1: expr t1) (e2: expr t2) S1 S2 :
         mac_safe sk e1 S1 ->
         mac_safe sk e2 S2 ->
@@ -1792,7 +1793,7 @@ Section Language.
     (* boring recursion: *)
     | esconst t v : @encrypt_safe sk t #v
     | esfunc {t1 t2} (f : func t1 t2) e : encrypt_safe sk e -> encrypt_safe sk (f@e)
-    | esadv                           e : encrypt_safe sk e -> encrypt_safe sk (!@e)
+    | esadv  {t1 t2} (e : expr t1) : encrypt_safe sk e -> encrypt_safe sk (!t2@e)
     | espair {t1 t2} (e1: expr t1) (e2: expr t2) :
         encrypt_safe sk e1 ->
         encrypt_safe sk e2 ->
@@ -1805,7 +1806,7 @@ Section Language.
     | encs_encrypt : encrypts sk n m (encrypt@(keygen@($sk), n, m))
     (* boring recursion: *)
     | encs_func {t1 t2} (f : func t1 t2) e : encrypts sk n m e -> encrypts sk n m (f@e)
-    | encs_adv                           e : encrypts sk n m e -> encrypts sk n m (!@e)
+    | encs_adv  {t1 t2} (e : expr t1) : encrypts sk n m e -> encrypts sk n m (!t2@e)
     | encs_pair_l {t1 t2} (e1 : expr t1) (e2 : expr t2) :
         encrypts sk n m e1 -> encrypts sk n m (e1, e2)
     | encs_pair_r {t1 t2} (e1 : expr t1) (e2 : expr t2) :
@@ -1828,7 +1829,7 @@ Section Language.
                    (encrypt@(keygen@($sk), n, m'))
     (* boring recursion: *)
     | eqe_func {t1 t2} (f : func t1 t2) e e' : eq_mod_enc sk e e' -> eq_mod_enc sk (f@e) (f@e')
-    | eqe_adv e e'                           : eq_mod_enc sk e e' -> eq_mod_enc sk (!@e) (!@e')
+    | eqe_adv {t1 t2} (e e' : expr t1) : eq_mod_enc sk e e' -> eq_mod_enc sk (!t2@e) (!t2@e')
     | eqe_pair {t1 t2} (e1 e1' : expr t1) (e2 e2' : expr t2) :
         eq_mod_enc sk e1 e1' ->
         eq_mod_enc sk e2 e2' ->
@@ -1888,7 +1889,7 @@ Section Language.
       (forall h, encrypt_safe sk (message h)) ->
       (forall {t} x, @P t (#x)%expr) -> (* WHY do we need a scope annotation here *)
       (forall idx, idx <> sk -> P ($idx)%expr) -> (* and here? *)
-      (forall e', P e' ->  P (!@e')) ->
+      (forall t1 t2 (e' : expr t1), P e' ->  P (!t2@e')) ->
       (forall t1 t2 (f : func t1 t2) e', encrypt_safe sk e' -> P e' -> P (f@e')) ->
       (forall t1 e1 t2 e2, @P t1 e1 -> @P t2 e2 -> P (e1, e2)%expr) -> (* and here? *)
       (forall h, P (encrypt@(keygen@($sk), nonce h, message h))) ->
@@ -2132,7 +2133,7 @@ Section Language.
       Definition mac_out := mac@(sk2, enc_out).
       Definition mmac_out := mac2message@mac_out.
       Definition net_in_1 := fcons@(enc_out, fcons@(mmac_out, #cnil)).
-      Definition adv_out_1 := !@net_in_1.
+      Definition adv_out_1 := !tmessage@net_in_1.
       Definition adv_out_1_tup := prod_decode@adv_out_1.
       Definition adv_out_msg := ffst@adv_out_1_tup.
       Definition adv_out_mmac := fsnd@adv_out_1_tup.
@@ -2155,7 +2156,7 @@ Section Language.
                               then net_in_good
                               else fcons@(#complaint, net_in_1))%expr.
 
-      Definition adv_out_2 := !@net_in_2.
+      Definition adv_out_2 := !tmessage@net_in_2.
       Definition adv_out_2_tup := prod_decode@adv_out_2.
       Definition adv_out_2_msg := ffst@adv_out_2_tup.
       Definition adv_out_2_sig_m := fsnd@adv_out_2_tup.
